proof/theories/Compile.v
@@ -105,6 +105,8 @@ Definition compile_vsrc (vs : vsrc) : list instr :=
   match vs with
   | VImm v      => [IImmediateData 1 v]
   | VField f ts => compile_load (field_load f) 1 :: compile_transforms ts
+  | VMap f name entries =>
+      [compile_load (field_load f) 1; ILookupVal 1 name 1 entries]
   end.
 
 Definition compile_stmt (s : stmt) : list instr :=
